theories/examples/region_macros.v
@@ -2,8 +2,7 @@ From iris.algebra Require Import frac.
 From iris.proofmode Require Import tactics.
 Require Import Eqdep_dec List.
 From cap_machine Require Import rules logrel.
-From cap_machine Require Export addr_reg_sample region_invariants_revocation
-     region_invariants_allocation multiple_updates.
+From cap_machine Require Export addr_reg_sample region_invariants_revocation multiple_updates.
 From cap_machine Require Export iris_extra.
 
 Section region_macros.
@@ -31,116 +30,116 @@ Section region_macros.
 
    (* -------------------- ALLOCATING A NEW REGION OF ZEROES ------------------ *)
 
-   Lemma region_addrs_zeroes_alloc_aux E a W p (n : nat) :
-     p ≠ O → is_Some (a + (Z.of_nat n))%a →
-     Forall (λ a, a ∉ dom (gset Addr) (std W)) (region_addrs_aux a n) →
-     ([∗ list] a0 ∈ region_addrs_aux a n, a0 ↦ₐ[p] inl 0%Z)
-       -∗ region W
-       -∗ sts_full_world W
-     ={E}=∗ ([∗ list] x ∈ region_addrs_aux a n, read_write_cond x p interp)
-         ∗ region (std_update_temp_multiple W (region_addrs_aux a n))
-         ∗ sts_full_world (std_update_temp_multiple W (region_addrs_aux a n)).
-   Proof.
-     iInduction (n) as [| n] "IHn" forall (a W).
-     - simpl. iIntros (_ _ _) "_ Hr Hsts". iFrame. done.
-     - iIntros (Hne Hnext Hforall) "Hlist Hr Hsts".
-       iDestruct "Hlist" as "[Ha Hlist]".
-       simpl in Hforall.
-       apply list.Forall_cons in Hforall as [ Hasta Hforall].
-       destruct (pwl p) eqn:Hpwl.
-       + iAssert (∀ W, interp W (inl 0%Z))%I as "#Hav".
-         { iIntros (W'). rewrite fixpoint_interp1_eq. eauto. }
-         (* if n is 0 we do not need to use IH *)
-         destruct n.
-         { simpl. iFrame.
-           iMod (extend_region_temp_pwl E _ a p (inl 0%Z) (λ Wv, interp Wv.1 Wv.2)
-                 with "[] Hsts Hr Ha Hav") as "(Hr & Ha & Hsts)"; auto.
-           { iModIntro. iIntros (W1 W2 Hrelated) "Hv /=". do 2 (rewrite fixpoint_interp1_eq /=). done. }
-           iFrame. done.
-         }
-         iMod ("IHn" with "[] [] [] Hlist Hr Hsts") as "(Hlist & Hr & Hsts)"; auto.
-         { iPureIntro. destruct Hnext as [? ?]. zify_addr; solve [ eauto | lia ]. }
-         iFrame. destruct Hnext as [e He]. assert (a ≠ addr_reg.top) by (intros ->; solve_addr).
-         iMod (extend_region_temp_pwl E _ a p (inl 0%Z) (λ Wv, interp Wv.1 Wv.2)
-                 with "[] Hsts Hr Ha Hav") as "(Hr & Ha & Hsts)"; auto.
-         { apply (std_update_multiple_dom_sta_i _ (S n) _ _ 1); auto; lia. }
-         { iModIntro. iIntros (W1 W2 Hrelated) "Hv /=". do 2 (rewrite fixpoint_interp1_eq /=). done. }
-         iFrame. done.
-       + iAssert (∀ W, interp W (inl 0%Z))%I as "#Hav".
-         { iIntros (W'). rewrite fixpoint_interp1_eq. eauto. }
-         (* if n is 0 we do not need to use IH *)
-         destruct n.
-         { simpl. iFrame.
-           iMod (extend_region_temp_nwl E _ a p (inl 0%Z) (λ Wv, interp Wv.1 Wv.2)
-                 with "[] Hsts Hr Ha Hav") as "(Hr & Ha & Hsts)"; auto.
-           { iModIntro. iIntros (W1 W2 Hrelated) "Hv /=". do 2 (rewrite fixpoint_interp1_eq /=). done. }
-           iFrame. done.
-         }
-         iMod ("IHn" with "[] [] [] Hlist Hr Hsts") as "(Hlist & Hr & Hsts)"; auto.
-         { iPureIntro. destruct Hnext as [? ?]. zify_addr; solve [ eauto | lia ]. }
-         iFrame. destruct Hnext as [e He]. assert (a ≠ addr_reg.top) by (intros ->; solve_addr).
-         iMod (extend_region_temp_nwl E _ a p (inl 0%Z) (λ Wv, interp Wv.1 Wv.2)
-                 with "[] Hsts Hr Ha Hav") as "(Hr & Ha & Hsts)"; auto.
-         { apply (std_update_multiple_dom_sta_i _ (S n) _ _ 1); auto; lia. }
-         { iModIntro. iIntros (W1 W2 Hrelated) "Hv /=". do 2 (rewrite fixpoint_interp1_eq /=). done. }
-         iFrame. done.
-   Qed.
+   (* Lemma region_addrs_zeroes_alloc_aux E a W p (n : nat) : *)
+   (*   p ≠ O → is_Some (a + (Z.of_nat n))%a → *)
+   (*   Forall (λ a, a ∉ dom (gset Addr) (std W)) (region_addrs_aux a n) → *)
+   (*   ([∗ list] a0 ∈ region_addrs_aux a n, a0 ↦ₐ[p] inl 0%Z) *)
+   (*     -∗ region W *)
+   (*     -∗ sts_full_world W *)
+   (*   ={E}=∗ ([∗ list] x ∈ region_addrs_aux a n, read_write_cond x p interp) *)
+   (*       ∗ region (std_update_temp_multiple W (region_addrs_aux a n)) *)
+   (*       ∗ sts_full_world (std_update_temp_multiple W (region_addrs_aux a n)). *)
+   (* Proof. *)
+   (*   iInduction (n) as [| n] "IHn" forall (a W). *)
+   (*   - simpl. iIntros (_ _ _) "_ Hr Hsts". iFrame. done. *)
+   (*   - iIntros (Hne Hnext Hforall) "Hlist Hr Hsts". *)
+   (*     iDestruct "Hlist" as "[Ha Hlist]". *)
+   (*     simpl in Hforall. *)
+   (*     apply list.Forall_cons in Hforall as [ Hasta Hforall]. *)
+   (*     destruct (pwl p) eqn:Hpwl. *)
+   (*     + iAssert (∀ W, interp W (inl 0%Z))%I as "#Hav". *)
+   (*       { iIntros (W'). rewrite fixpoint_interp1_eq. eauto. } *)
+   (*       (* if n is 0 we do not need to use IH *) *)
+   (*       destruct n. *)
+   (*       { simpl. iFrame. *)
+   (*         iMod (extend_region_temp_pwl E _ a p (inl 0%Z) (λ Wv, interp Wv.1 Wv.2) *)
+   (*               with "[] Hsts Hr Ha Hav") as "(Hr & Ha & Hsts)"; auto. *)
+   (*         { iModIntro. iIntros (W1 W2 Hrelated) "Hv /=". do 2 (rewrite fixpoint_interp1_eq /=). done. } *)
+   (*         iFrame. done. *)
+   (*       } *)
+   (*       iMod ("IHn" with "[] [] [] Hlist Hr Hsts") as "(Hlist & Hr & Hsts)"; auto. *)
+   (*       { iPureIntro. destruct Hnext as [? ?]. zify_addr; solve [ eauto | lia ]. } *)
+   (*       iFrame. destruct Hnext as [e He]. assert (a ≠ addr_reg.top) by (intros ->; solve_addr). *)
+   (*       iMod (extend_region_temp_pwl E _ a p (inl 0%Z) (λ Wv, interp Wv.1 Wv.2) *)
+   (*               with "[] Hsts Hr Ha Hav") as "(Hr & Ha & Hsts)"; auto. *)
+   (*       { apply (std_update_multiple_dom_sta_i _ (S n) _ _ 1); auto; lia. } *)
+   (*       { iModIntro. iIntros (W1 W2 Hrelated) "Hv /=". do 2 (rewrite fixpoint_interp1_eq /=). done. } *)
+   (*       iFrame. done. *)
+   (*     + iAssert (∀ W, interp W (inl 0%Z))%I as "#Hav". *)
+   (*       { iIntros (W'). rewrite fixpoint_interp1_eq. eauto. } *)
+   (*       (* if n is 0 we do not need to use IH *) *)
+   (*       destruct n. *)
+   (*       { simpl. iFrame. *)
+   (*         iMod (extend_region_temp_nwl E _ a p (inl 0%Z) (λ Wv, interp Wv.1 Wv.2) *)
+   (*               with "[] Hsts Hr Ha Hav") as "(Hr & Ha & Hsts)"; auto. *)
+   (*         { iModIntro. iIntros (W1 W2 Hrelated) "Hv /=". do 2 (rewrite fixpoint_interp1_eq /=). done. } *)
+   (*         iFrame. done. *)
+   (*       } *)
+   (*       iMod ("IHn" with "[] [] [] Hlist Hr Hsts") as "(Hlist & Hr & Hsts)"; auto. *)
+   (*       { iPureIntro. destruct Hnext as [? ?]. zify_addr; solve [ eauto | lia ]. } *)
+   (*       iFrame. destruct Hnext as [e He]. assert (a ≠ addr_reg.top) by (intros ->; solve_addr). *)
+   (*       iMod (extend_region_temp_nwl E _ a p (inl 0%Z) (λ Wv, interp Wv.1 Wv.2) *)
+   (*               with "[] Hsts Hr Ha Hav") as "(Hr & Ha & Hsts)"; auto. *)
+   (*       { apply (std_update_multiple_dom_sta_i _ (S n) _ _ 1); auto; lia. } *)
+   (*       { iModIntro. iIntros (W1 W2 Hrelated) "Hv /=". do 2 (rewrite fixpoint_interp1_eq /=). done. } *)
+   (*       iFrame. done. *)
+   (* Qed. *)
 
-   Lemma region_addrs_zeroes_valid_aux n W :
-     ⊢ ([∗ list] y ∈ replicate n (inl 0%Z), ▷ (fixpoint interp1) W y).
-   Proof.
-     iInduction (n) as [| n] "IHn".
-     - done.
-     - simpl. iSplit; last iFrame "#".
-       rewrite fixpoint_interp1_eq. iNext.
-       eauto.
-   Qed.
+   (* Lemma region_addrs_zeroes_valid_aux n W : *)
+   (*   ⊢ ([∗ list] y ∈ replicate n (inl 0%Z), ▷ (fixpoint interp1) W y). *)
+   (* Proof. *)
+   (*   iInduction (n) as [| n] "IHn". *)
+   (*   - done. *)
+   (*   - simpl. iSplit; last iFrame "#". *)
+   (*     rewrite fixpoint_interp1_eq. iNext. *)
+   (*     eauto. *)
+   (* Qed. *)
 
-   Lemma region_addrs_zeroes_valid (a b : Addr) W :
-     ⊢ ([∗ list] _;y2 ∈ region_addrs a b; region_addrs_zeroes a b,
-                                        ▷ (fixpoint interp1) W y2).
-   Proof.
-     rewrite /region_addrs /region_addrs_zeroes.
-     iApply (big_sepL2_to_big_sepL_r _ _ (region_addrs_zeroes a b)).
-     - rewrite region_addrs_aux_length replicate_length //.
-     - iApply region_addrs_zeroes_valid_aux.
-   Qed.
+   (* Lemma region_addrs_zeroes_valid (a b : Addr) W : *)
+   (*   ⊢ ([∗ list] _;y2 ∈ region_addrs a b; region_addrs_zeroes a b, *)
+   (*                                      ▷ (fixpoint interp1) W y2). *)
+   (* Proof. *)
+   (*   rewrite /region_addrs /region_addrs_zeroes. *)
+   (*   iApply (big_sepL2_to_big_sepL_r _ _ (region_addrs_zeroes a b)). *)
+   (*   - rewrite region_addrs_aux_length replicate_length //. *)
+   (*   - iApply region_addrs_zeroes_valid_aux. *)
+   (* Qed. *)
 
-   Lemma region_addrs_zeroes_trans_aux (a b : Addr) p n :
-     ([∗ list] y1;y2 ∈ region_addrs_aux a n;replicate n (inl 0%Z), y1 ↦ₐ[p] y2)
-       -∗ [∗ list] y1 ∈ region_addrs_aux a n, y1 ↦ₐ[p] inl 0%Z.
-   Proof.
-     iInduction (n) as [| n] "IHn" forall (a); first auto.
-     iIntros "Hlist".
-     iDestruct "Hlist" as "[Ha Hlist]".
-     iFrame.
-     iApply "IHn". iFrame.
-   Qed.
+   (* Lemma region_addrs_zeroes_trans_aux (a b : Addr) p n : *)
+   (*   ([∗ list] y1;y2 ∈ region_addrs_aux a n;replicate n (inl 0%Z), y1 ↦ₐ[p] y2) *)
+   (*     -∗ [∗ list] y1 ∈ region_addrs_aux a n, y1 ↦ₐ[p] inl 0%Z. *)
+   (* Proof. *)
+   (*   iInduction (n) as [| n] "IHn" forall (a); first auto. *)
+   (*   iIntros "Hlist". *)
+   (*   iDestruct "Hlist" as "[Ha Hlist]". *)
+   (*   iFrame. *)
+   (*   iApply "IHn". iFrame. *)
+   (* Qed. *)
 
-   Lemma region_addrs_zeroes_trans (a b : Addr) p :
-     ([∗ list] y1;y2 ∈ region_addrs a b;region_addrs_zeroes a b, y1 ↦ₐ[p] y2)
-       -∗ [∗ list] a0 ∈ region_addrs a b, a0 ↦ₐ[p] (inl 0%Z).
-   Proof.
-     iIntros "Hlist".
-     rewrite /region_addrs /region_addrs_zeroes.
-     iApply region_addrs_zeroes_trans_aux; auto.
-   Qed.
+   (* Lemma region_addrs_zeroes_trans (a b : Addr) p : *)
+   (*   ([∗ list] y1;y2 ∈ region_addrs a b;region_addrs_zeroes a b, y1 ↦ₐ[p] y2) *)
+   (*     -∗ [∗ list] a0 ∈ region_addrs a b, a0 ↦ₐ[p] (inl 0%Z). *)
+   (* Proof. *)
+   (*   iIntros "Hlist". *)
+   (*   rewrite /region_addrs /region_addrs_zeroes. *)
+   (*   iApply region_addrs_zeroes_trans_aux; auto. *)
+   (* Qed. *)
 
-   Lemma region_addrs_zeroes_alloc E W (a b : Addr) p :
-     p ≠ O →
-     Forall (λ a0 : Addr, (a0 ∉ dom (gset Addr) (std W))) (region_addrs a b) →
-     ([∗ list] y1;y2 ∈ region_addrs a b;region_addrs_zeroes a b, y1 ↦ₐ[p] y2)
-       ∗ region W ∗ sts_full_world W
-     ={E}=∗ ([∗ list] a0 ∈ region_addrs a b, read_write_cond a0 p interp)
-         ∗ region (std_update_temp_multiple W (region_addrs a b))
-         ∗ sts_full_world (std_update_temp_multiple W (region_addrs a b)).
-   Proof.
-     iIntros (Hne Hforall) "[Hlist [Hr Hsts] ]".
-     iDestruct (region_addrs_zeroes_trans with "Hlist") as "Hlist".
-     rewrite /region_addrs. rewrite /region_addrs in Hforall.
-     iMod (region_addrs_zeroes_alloc_aux with "[$Hlist] [$Hr] [$Hsts]") as "H"; auto.
-     rewrite /region_size. zify_addr; eauto; lia.
-   Qed.
+   (* Lemma region_addrs_zeroes_alloc E W (a b : Addr) p : *)
+   (*   p ≠ O → *)
+   (*   Forall (λ a0 : Addr, (a0 ∉ dom (gset Addr) (std W))) (region_addrs a b) → *)
+   (*   ([∗ list] y1;y2 ∈ region_addrs a b;region_addrs_zeroes a b, y1 ↦ₐ[p] y2) *)
+   (*     ∗ region W ∗ sts_full_world W *)
+   (*   ={E}=∗ ([∗ list] a0 ∈ region_addrs a b, read_write_cond a0 p interp) *)
+   (*       ∗ region (std_update_temp_multiple W (region_addrs a b)) *)
+   (*       ∗ sts_full_world (std_update_temp_multiple W (region_addrs a b)). *)
+   (* Proof. *)
+   (*   iIntros (Hne Hforall) "[Hlist [Hr Hsts] ]". *)
+   (*   iDestruct (region_addrs_zeroes_trans with "Hlist") as "Hlist". *)
+   (*   rewrite /region_addrs. rewrite /region_addrs in Hforall. *)
+   (*   iMod (region_addrs_zeroes_alloc_aux with "[$Hlist] [$Hr] [$Hsts]") as "H"; auto. *)
+   (*   rewrite /region_size. zify_addr; eauto; lia. *)
+   (* Qed. *)
 
 
    (* ------------------------------ OPENING A REGION ----------------------------------- *)
